Tests.lean
@@ -5,6 +5,7 @@ Authors: Bangyen Pham
 -/
 import Tests.Compiler
 import Tests.Completeness
+import Tests.Examples
 import Tests.Minsky
 import Tests.Semantics
 import Tests.State
